formal/lean4/L4Factoidal.lean
@@ -90,6 +90,7 @@ import L4Factoidal.Syntax.NQuadsFastTheorems
 import L4Factoidal.Syntax.LexShift
 import L4Factoidal.Syntax.IriResolve
 import L4Factoidal.Syntax.Turtle
+import L4Factoidal.Syntax.TurtleFuelTheorems
 import L4Factoidal.Syntax.TurtleSerialize
 import L4Factoidal.Syntax.TriG
 import L4Factoidal.Syntax.TurtleTests
